For the general quadratic equation, \(ax^2+bx+c=0,\) the solutions (there can be \(2, \ 1\) or \(0\) real number solutions) are
\[x = \frac{-b\pm \sqrt{b^2-4ac}}{2a}.\]

\begin{question}
    Solve for \(x:\) \(2x^2+\frac{3}{2}x-3=0.\)
    \begin{expandable}{}{}
        \begin{solution}
            \begin{flalign*}
                x&=\frac{-3/2 \pm \sqrt{9/4-4\left(2\right)\left(-3\right)}}{2\left(2\right)} \\
                &= \frac{-3/2 \pm \sqrt{9/4+24}}{4} \\
                &= \frac{2}{2}\frac{-3/2 \pm \sqrt{9/4 +24}}{4} \\
                &= \frac{-3 \pm \sqrt{9+24\left(4\right)}}{8} \\
                &= \frac{-3 \pm \sqrt{105}}{8}
            \end{flalign*}
            The complete set of solutions to our equation is \(\{\frac{-3+\sqrt{105}}{8},\frac{-3-\sqrt{105}}{8}\}.\)
        \end{solution}
    \end{expandable}
\end{question}

\begin{question}
    Solve for \(z:\) \(2z^2+z+3=0.\)
    \begin{expandable}{}{}
        \begin{solution}
            \begin{flalign*}
                z&=\frac{-1 \pm \sqrt{1-4\left(2\right)\left(3\right)}}{2\left(2\right)} \\
                &= \frac{-1 \pm \sqrt{-23}}{4}
            \end{flalign*}
            Since \(\sqrt{-23}\) is not a real number, there are no solutions to this equation!

            The set of real solutions is \(\emptyset.\)

            This is the empty set. The set which has no elements.
        \end{solution}
    \end{expandable}
\end{question}